updates

src/Common.v
@@ -119,3 +119,472 @@ Qed.
 Tactic Notation "buint_all" := (repeat (rewrite buint2 || rewrite buint1 || rewrite buint0)).
 
 Tactic Notation "buint_all" "in" hyp(H) := (repeat (rewrite buint2 in H || rewrite buint1 in H || rewrite buint0 in H)).
+
+
+Check fold_left.
+
+Definition hmapSum {K} (m: mapping K N) := 
+match m with 
+| wrap _ l => fold_left (fun s x => snd x + s) l 0
+end.
+
+Search fold_left.
+
+Lemma fold_left_addable: forall X (l: Datatypes.list X) a (f: X -> N ),
+      fold_left (fun s x => f x + s) l a = a + fold_left (fun s x => f x + s) l 0.
+Proof.
+  intros. generalize dependent a.
+  induction l; intros.
+  - simpl. lia.
+  - simpl. rewrite IHl. symmetry.
+  rewrite IHl. lia.
+Qed.
+
+Check BoolEq.eqb_spec.
+
+Import ListNotations.
+
+Lemma hmapSumDelete: forall {K}`{XBoolEquable bool K}`{BoolEq.eqb_spec K} (m: mapping K N) k, 
+keysDistinct m ->
+hmapSum m = m [k] + hmapSum (deleteListPair k m).
+Proof.
+intros.
+destruct m. induction l.
+- auto.
+- unfold Common.hmapFindWithDefault. unfold hmapLookup.
+  simpl. destruct a. simpl. remember (eqb k k0).
+  case_eq y; intros.
+  + simpl. rewrite fold_left_addable.
+  setoid_rewrite IHl.  
+  rewrite lookup_none_find. unfold Datatypes.id. simpl default. 
+  unfold hmapSum. simpl. lia.
+  rewrite <- keysDistinct_cons_lookup_none with (t:=n). auto.
+  destruct H0. rewrite H2 in Heqy. symmetry in Heqy.
+  apply eqb_spec_intro in Heqy. rewrite Heqy. assumption.
+  enough (keysDistinct_list ((([ (k0, n) ])%list ++ l))%list).
+  apply keysDistinct_app in H3.
+  tauto. apply H1.
+  + simpl. rewrite fold_left_addable.
+    symmetry. rewrite fold_left_addable.
+    setoid_rewrite IHl.
+    unfold Common.hmapFindWithDefault. unfold hmapLookup.
+    simpl. lia.
+    enough (keysDistinct_list ((([ (k0, n) ])%list ++ l))%list).
+    apply keysDistinct_app in H3.
+    tauto. apply H1.
+Qed.
+
+
+Lemma hmapSumEqual: forall {K}`{XBoolEquable bool K}`{BoolEq.eqb_spec K} (m1 m2: mapping K N), keysDistinct m1 -> keysDistinct m2 -> (forall k, m1[k] = m2[k]) -> 
+hmapSum m1 = hmapSum m2.
+Proof.
+intros.
+destruct m1, m2.
+generalize dependent l0.
+induction l; intros.
+- simpl. simpl in H3. unfold Common.hmapFindWithDefault at 1 in H3.
+  simpl in H3. induction l0.
+  + auto.
+  + simpl. rewrite fold_left_addable.
+    rewrite <- IHl0.
+    enough (snd a = 0). lia. 
+    pose proof (H3 (fst a)).
+    unfold Common.hmapFindWithDefault in H4.
+    simpl in H4. unfold hmapLookup in H4.
+    simpl in H4. destruct H0.
+    replace (eqb (fst a) (fst a)) with true in H4.
+    simpl in H4. auto. symmetry.
+    apply eqb_spec_intro. auto.
+    enough (keysDistinct_list ((([ a ])%list ++ l0))%list).
+    apply keysDistinct_app in H4.
+    tauto. apply H2. intros.    
+    unfold Common.hmapFindWithDefault in H3.
+    simpl in H3. unfold hmapLookup in H3.
+    simpl in H3. pose proof (H3 k).
+    remember (eqb k (fst a)).
+    case_eq y; intros.
+    * rewrite H5 in H4. simpl in H4.
+      rewrite lookup_none_find. auto.
+      rewrite <- keysDistinct_cons_lookup_none with (t:=snd a). auto.
+      destruct a. simpl. simpl in Heqy. 
+      rewrite H5 in Heqy. symmetry in Heqy. 
+      destruct H0.
+      apply eqb_spec_intro in Heqy. rewrite Heqy.
+      assumption.
+    * rewrite H5 in H4. setoid_rewrite <- H4. auto.
+- remember (deleteListPair (fst a) (wrap Map l0)).
+  enough (forall k : K, (wrap Map l) [k] = l1 [k]).      
+  enough (hmapSum (wrap Map (a :: l)) = snd a + hmapSum (wrap Map l)).
+  rewrite H5. destruct l1. rewrite IHl with (l0:=l1).
+  rewrite Heql1. symmetry.
+  rewrite hmapSumDelete with (k:=fst a).
+  pose proof (H3 (fst a)).
+  simpl in H6.  unfold Common.hmapFindWithDefault in H6.
+  unfold hmapLookup in H6.
+  simpl in H6. replace (eqb (fst a) (fst a)) with true in H6.
+  simpl in H6. setoid_rewrite <- H6.
+  auto.
+  destruct H0. symmetry. apply eqb_spec_intro. auto.
+  assumption.
+  enough (keysDistinct_list ((([ a ])%list ++ l))%list).
+  apply keysDistinct_app in H6.
+  tauto. apply H1.
+  rewrite Heql1. apply delete_kd. assumption.
+  assumption.
+  simpl. rewrite fold_left_addable. lia.
+  intros. rewrite Heql1.
+  remember (eqb k (fst a)).
+  case_eq y; intros.
+  + rewrite H4 in Heqy. symmetry in Heqy.
+    destruct H0. apply eqb_spec_intro in Heqy.
+    rewrite ?lookup_none_find. auto. rewrite Heqy.
+    rewrite lookup_delete_none. auto.
+    erewrite <- keysDistinct_cons_lookup_none with (t:=snd a). auto.
+    destruct a. simpl. rewrite Heqy. apply H1.
+  + remember ((wrap Map l0) [k]?). pose proof (H3 k).
+    unfold Common.hmapFindWithDefault in H5.
+    unfold hmapLookup in H5. simpl in H5.
+    rewrite H4 in Heqy. rewrite <- Heqy in H5.
+    unfold Common.hmapFindWithDefault.
+    rewrite lookup_delete_another.  
+    assumption.
+    unfold not. intros.
+    symmetry in H6. destruct H0. apply eqb_spec_intro in H6.
+    rewrite H6 in Heqy.
+    discriminate.
+    Unshelve. split; assumption.   
+Qed.
+
+
+Lemma hmapSumAdjust: forall {K}`{XBoolEquable bool K}`{BoolEq.eqb_spec K} (m: mapping K N) k a, 
+keysDistinct m ->
+hmapSum (m[k] ← a) = a + hmapSum m - m[k].
+Proof.
+intros. rewrite hmapSumDelete with (k:=k).
+symmetry. rewrite hmapSumDelete with (k:=k).
+symmetry.
+rewrite lookup_some_find with (v:=a).
+(* remember (deleteListPair k m). *)
+rewrite delete_insert. lia.
+rewrite lookup_addAdjust with (v:=a). auto.
+assumption.
+apply insert_kd.
+assumption.
+Qed.
+
+
+Check (* FinProof.MonadTransformers21. *)TransEmbedded.    
+Check LedgerLEmbeddedType.
+Print ContractFields.
+
+Check (@TransEmbedded _ _ _ (LedgerLEmbeddedType rec Ledger_MainState) 
+                            (ContractLEmbeddedType _decimals) ).
+
+
+Definition mappingProj {K V}`{XBoolEquable bool K}`{XDefault V} (k: K) (m: mapping K V) : V := m[k].
+Definition mappingInj {K V}`{XBoolEquable bool K} (k: K) (v: V) (m: mapping K V) : mapping K V :=  m[k] ← v.
+
+Check projinj.
+
+Transparent Common.hmapFindWithDefault
+        CommonInstances.addAdjustListPair
+        N.add N.sub N.leb N.ltb N.eqb Z.eqb.
+
+Lemma mappingProjInj: forall {K V}`{XBoolEquable bool K}`{BoolEq.eqb_spec K}`{XDefault V}  (k: K) (v: V) (m: mapping K V), 
+                      mappingProj k (mappingInj k v m) = v.
+Proof.
+  intros.
+  unfold mappingInj, mappingProj.
+  rewrite lookup_some_find with (v:=v). auto.
+  unshelve erewrite lookup_addAdjust with (k:=k). auto.
+Qed.
+
+Lemma mappingInjProj: forall {K V}`{XBoolEquable bool K}`{BoolEq.eqb_spec K}`{XDefault V} (k: K) (m: mapping K V), 
+keysDistinct m ->
+mappingInj k (mappingProj k m) m = m.
+Proof.
+  intros.
+  unfold mappingInj, mappingProj.  
+  - case_eq (m [k] ?); intros.
+  + rewrite lookup_some_find with (v:=v).
+    (* rewrite lookup_some_find with (v:=v). *)
+    unfold xHMapInsert. simpl. destruct m.
+    apply member_addAdjust. assumption. assumption. assumption.
+  + admit.
+Admitted.  
+
+Check injinj.
+
+Lemma mappingInjInj: forall {K V}`{XBoolEquable bool K}`{BoolEq.eqb_spec K} (k: K) (v1 v2: V) (m: mapping K V), 
+(* keysDistinct m -> *)
+mappingInj k v1 (mappingInj k v2 m) = mappingInj k v1 m.
+Proof.
+  intros.
+  unfold mappingInj.  
+  rewrite insert_insert. auto.
+Qed.
+
+Obligation Tactic := intros.
+
+#[global]
+Program Instance mapping_embedded: forall {K V}`{XBoolEquable bool K}`{BoolEq.eqb_spec K}`{XDefault V} (k: K),
+EmbeddedType (mapping K V) V | 0.
+Next Obligation.
+apply mappingProj. exact k. exact X.
+Defined.
+Next Obligation.
+apply mappingInj. exact k. exact X. exact X0.
+Defined.
+Next Obligation.
+unfold mapping_embedded_obligation_1, mapping_embedded_obligation_2.
+apply mappingProjInj.
+Defined.
+Next Obligation.
+unfold mapping_embedded_obligation_1, mapping_embedded_obligation_2.
+apply mappingInjProj.
+admit.
+Admitted.
+Next Obligation.
+unfold mapping_embedded_obligation_1, mapping_embedded_obligation_2.
+apply mappingInjInj.
+Defined.
+Fail Next Obligation.
+
+
+(* Definition mappingProj {K V}`{XBoolEquable bool K} (k: K) (m: mapping K V) : option V := m[k]?.
+Definition mappingInj {K V}`{XBoolEquable bool K} (k: K) (ov: option V) (m: mapping K V) : mapping K V := 
+match ov with 
+| None => deleteListPair k m
+| Some v => m[k] ← v
+end.
+
+Check projinj.
+
+Transparent Common.hmapFindWithDefault
+        CommonInstances.addAdjustListPair
+        N.add N.sub N.leb N.ltb N.eqb Z.eqb.
+
+Lemma mappingProjInj: forall {K V}`{XBoolEquable bool K}`{BoolEq.eqb_spec K} (k: K) (ov: option V) (m: mapping K V), 
+                      mappingProj k (mappingInj k ov m) = ov.
+Proof.
+  intros.
+  unfold mappingInj, mappingProj.
+  destruct ov.
+  - unshelve erewrite lookup_addAdjust with (k:=k). auto.
+  - unshelve erewrite lookup_delete_none with (k:=k). auto.
+Qed.
+
+
+Lemma mappingInjProj: forall {K V}`{XBoolEquable bool K}`{BoolEq.eqb_spec K} (k: K) (m: mapping K V), 
+keysDistinct m ->
+mappingInj k (mappingProj k m) m = m.
+Proof.
+  intros.
+  unfold mappingInj, mappingProj.  
+  - case_eq (m [k] ?); intros.
+  + destruct m.
+    apply member_addAdjust. assumption. assumption.
+  + unfold deleteListPair. rewrite delete_not_member_list.
+    destruct m. auto. assumption. 
+Qed.  
+
+Check injinj.
+
+Lemma mappingInjInj: forall {K V}`{XBoolEquable bool K}`{BoolEq.eqb_spec K} (k: K) (ov1 ov2: option V) (m: mapping K V), 
+(* keysDistinct m -> *)
+mappingInj k ov1 (mappingInj k ov2 m) = mappingInj k ov1 m.
+Proof.
+  intros.
+  unfold mappingInj.
+  destruct ov1, ov2.
+  - rewrite insert_insert. auto.
+  - remember (m[k]?).
+    destruct y.
+    + admit.
+    + unfold deleteListPair. rewrite delete_not_member_list.
+      auto. auto.
+  - unfold xHMapInsert. simpl.
+    rewrite delete_insert. auto.
+  - rewrite delete_not_member. auto.
+    rewrite lookup_delete_none.
+    auto.
+Admitted. *)
+
+(* Obligation Tactic := intros.
+
+#[global]
+Program Instance mapping_embedded: forall {K V}`{XBoolEquable bool K}`{BoolEq.eqb_spec K} (k: K),
+EmbeddedType (mapping K V) (option V).
+Next Obligation.
+apply mappingProj. exact k. exact X.
+Defined.
+Next Obligation.
+apply mappingInj. exact k. exact X. exact X0.
+Defined.
+Next Obligation.
+unfold mapping_embedded_obligation_1, mapping_embedded_obligation_2.
+apply mappingProjInj.
+Defined.
+Next Obligation.
+unfold mapping_embedded_obligation_1, mapping_embedded_obligation_2.
+apply mappingInjProj.
+admit.
+Admitted.
+Next Obligation.
+unfold mapping_embedded_obligation_1, mapping_embedded_obligation_2.
+apply mappingInjInj.
+Defined.
+Fail Next Obligation.
+
+Definition mappingOptProj {K V}`{XBoolEquable bool K} (k: K) (om: option (mapping K V)) : option V := 
+match om with
+| Some m => m[k]?
+| None => None
+end.
+
+Definition mappingOptInj {K V}`{XBoolEquable bool K} (k: K) (ov: option V) (om: option (mapping K V)) : option (mapping K V) := 
+match ov, om with 
+| None, None => None
+| None, Some m => Some (deleteListPair k m)
+| Some v, None => (* Some (default[k] ← v) *) None
+| Some v, Some m => Some (m[k] ← v)
+end.
+
+Lemma mappingOptProjInj: forall {K V}`{XBoolEquable bool K}`{BoolEq.eqb_spec K} (k: K) (ov: option V) (om: option(mapping K V)), 
+                      mappingOptProj k (mappingOptInj k ov om) = ov.
+Proof.
+  intros.
+  unfold mappingOptInj, mappingOptProj.
+  destruct ov, om.
+  - unshelve erewrite lookup_addAdjust with (k:=k). auto.
+  - unshelve erewrite lookup_addAdjust with (k:=k). auto.
+  - unshelve erewrite lookup_delete_none with (k:=k). auto.
+  - auto.
+Qed.
+
+Lemma mappingOptInjProj: forall {K V}`{XBoolEquable bool K}`{BoolEq.eqb_spec K} (k: K) (om: option(mapping K V)), 
+(match om with
+ | None => True
+ | Some m => keysDistinct m
+end) ->
+mappingOptInj k (mappingOptProj k om) om = om.
+Proof.
+  intros.
+  unfold mappingOptInj, mappingOptProj. 
+  destruct om; [|auto].
+  - case_eq (x [k] ?); intros.
+  + f_equal. destruct x.
+    apply member_addAdjust. assumption. assumption.
+  + f_equal. unfold deleteListPair. rewrite delete_not_member_list.
+    destruct x. auto. assumption. 
+  (* - exfalso. assumption.   *)
+Qed.  
+
+Lemma mappinOptgInjInj: forall {K V}`{XBoolEquable bool K}`{BoolEq.eqb_spec K} (k: K) (ov1 ov2: option V) 
+  (om: option(mapping K V)), 
+(* keysDistinct m -> *)
+mappingOptInj k ov1 (mappingOptInj k ov2 om) = mappingOptInj k ov1 om.
+Proof.
+  intros.
+  unfold mappingOptInj.
+  destruct ov1, ov2, om; auto.
+  - rewrite insert_insert. auto.
+  - f_equal. rewrite insert_insert. auto.
+  - f_equal. remember (x[k]?).
+    destruct y.
+    + admit.
+    + unfold deleteListPair. rewrite delete_not_member_list.
+      auto. auto.
+  - f_equal. unfold xHMapInsert. simpl.
+    rewrite delete_insert. auto.
+  - f_equal. unfold xHMapInsert. simpl.
+    rewrite delete_insert. auto.
+  - f_equal. rewrite delete_not_member. auto.
+    rewrite lookup_delete_none.
+    auto.
+Admitted.
+
+#[global]
+Program Instance opt_mapping_embedded: forall {K V}`{XBoolEquable bool K}`{BoolEq.eqb_spec K} (k: K),
+EmbeddedType (option(mapping K V)) (option V).
+Next Obligation.
+apply mappingOptProj. exact k. exact X.
+Defined.
+Next Obligation.
+apply mappingOptInj. exact k. exact X. exact X0.
+Defined.
+Next Obligation.
+unfold opt_mapping_embedded_obligation_1, opt_mapping_embedded_obligation_2.
+apply mappingOptProjInj.
+Defined.
+Next Obligation.
+unfold opt_mapping_embedded_obligation_1, opt_mapping_embedded_obligation_2.
+apply mappingOptInjProj.
+admit.
+Admitted.
+Next Obligation.
+unfold mapping_embedded_obligation_1, mapping_embedded_obligation_2.
+apply mappingInjInj.
+Defined.
+Fail Next Obligation. *)
+
+Notation "':>' f , g" := (@TransEmbedded _ _ _ (_ f: EmbeddedType _ _) (_ g: EmbeddedType _ _)) (at level 20, only parsing).
+Notation "':>' 'μ' f , g" := (@TransEmbedded _ _ _ (mapping_embedded f: EmbeddedType _ _) (_ g: EmbeddedType _ _)) (at level 20, only parsing).
+Notation "':>' f , 'μ' g" := (@TransEmbedded _ _ _ (_ f: EmbeddedType _ _) (mapping_embedded g: EmbeddedType _ _)) (at level 20, only parsing).
+Notation "':>' 'μ' f , 'μ' g" := (@TransEmbedded _ _ _ (mapping_embedded f: EmbeddedType _ _) (mapping_embedded g: EmbeddedType _ _)) (at level 20, only parsing).
+
+Notation "v '-->' r 'with' et":= (@injEmbed _ _ et v r) (at level 22, only parsing).
+Notation "'<--' r 'with' et":= (@projEmbed _ _ et r) (at level 22, only parsing).
+
+Check :> Ledger_VMState , :> VMState_ι_msg_sender , add_std_ι_address.
+
+Check default --> (_:LedgerLRecord rec) with :> Ledger_VMState , :> VMState_ι_msg_sender , add_std_ι_address.
+Compute field_type add_std_ι_address.
+Check ((<-- (_:LedgerLRecord rec) with :> Ledger_VMState , :> VMState_ι_msg_sender , add_std_ι_address) : field_type add_std_ι_address) : uint256.
+
+Check 5: uint256.
+Check (0%Z, 8: uint256): address.
+Check mapping_embedded  ((0%Z, 8: uint256): address).
+(* Check :> _balances , ((0%Z, 8: uint256): address). *)
+Check ((5:uint256)) --> (_:LedgerLRecord rec) 
+      with :> Ledger_MainState , :> _balances , ((0%Z, 8: uint256): address).
+
+Compute ((5:uint256)) --> (default:LedgerLRecord rec) 
+      with :> Ledger_MainState , :> _balances , ((0%Z, 8: uint256): address).      
+
+Set Typeclasses Debug.
+Unset Typeclasses Iterative Deepening.
+
+Check _ _allowed: EmbeddedType _ _.
+Print ContractLEmbeddedType.
+Check _ _allowed: EmbeddedType _ (field_type _allowed).
+
+Check TransEmbedded. 
+Arguments TransEmbedded {S} {T} {U} & _ _.
+
+Check @TransEmbedded ContractLRecord _ _ (_ _allowed: EmbeddedType _ _)   (mapping_embedded (_:address)).
+Check  :> Ledger_MainState, :> _allowed , :> μ (_: address) , μ (_: address).      
+
+
+Notation "l :: f , g <-- v" := (@injEmbed _ _ (@TransEmbedded _ _ _ (_ f: EmbeddedType _ _) (_ g: EmbeddedType _ _)) v l) (at level 20, only parsing).
+Notation "l :: 'μ' f , g <-- v" := (@injEmbed _ _ (@TransEmbedded _ _ _ (mapping_embedded f: EmbeddedType _ _) (_ g: EmbeddedType _ _)) v l) (at level 20, only parsing).
+Notation "l :: f , 'μ' g <-- v" := (@injEmbed _ _ (@TransEmbedded _ _ _ (_ f: EmbeddedType _ _) (mapping_embedded g: EmbeddedType _ _)) v l) (at level 20, only parsing).
+Notation "l :: 'μ' f , 'μ' g <-- v" := (@injEmbed _ _ (@TransEmbedded _ _ _ (mapping_embedded f: EmbeddedType _ _) (mapping_embedded g: EmbeddedType _ _)) v l) (at level 20, only parsing).
+
+(* Notation "v '-->' r 'with' et":= (@injEmbed _ _ et v r) (at level 22, only parsing). *)
+Notation "'<--' r 'with' et":= (@projEmbed _ _ et r) (at level 22, only parsing).
+
+Check (default:LedgerLRecord rec) :: Ledger_MainState , _allowed <-- _.
+
+Compute (4:uint256) --> 
+      ((5:uint256) --> (default:LedgerLRecord rec) 
+      with :> Ledger_MainState , :> _allowed , :> μ ((0%Z, 8: uint256): address), μ ((0%Z, 8: uint256): address)) 
+      with :> Ledger_MainState , :> _allowed , :> μ ((0%Z, 7: uint256): address), μ ((0%Z, 6: uint256): address).      
+
+(* Check :> Ledger_MainState , 
+              :> _allowed , (_: address).  *)     
+
+(* Check ((5:uint256) ) --> (_:LedgerLRecord rec) 
+      with :> Ledger_MainState , 
+              :> _allowed ,               
+                  :> ((0%Z, 8: uint256): address), ((0%Z, 8: uint256): address).    *)   
